Add unsafe dynarray implementation.

theories/std/dynarray.v
@@ -1,19 +1,13 @@
 From ml Require Import
   prelude.
-From ml.bi Require Import
-  big_op.
 From ml.language Require Import
   notations
   proofmode.
 From ml.std Require Export
   base.
 From ml.std Require Import
-  diverge
-  assume
   record2
   math
-  reference
-  opt
   array.
 
 Section heapGS.
@@ -21,7 +15,7 @@ Section heapGS.
 
   Implicit Types b : bool.
   Implicit Types i : nat.
-  Implicit Types l r : loc.
+  Implicit Types l : loc.
   Implicit Types v t fn : val.
   Implicit Types vs : list val.
 
@@ -31,7 +25,7 @@ Section heapGS.
   Notation "t '.[data]'" := t.[1]%stdpp
   ( at level 5
   ) : stdpp_scope.
-  Notation "t '.[size]'" := t.[0]%E
+Notation "t '.[size]'" := t.[0]%E
   ( at level 5
   ) : expr_scope.
   Notation "t '.[data]'" := t.[1]%E
@@ -44,27 +38,15 @@ Section heapGS.
 
   Definition dynarray_make : val :=
     λ: "sz" "v",
-      assume (#0 ≤ "sz") ;;
-      record2_make "sz" (array_init "sz" (λ: <>, &Some (ref "v"))).
+      record2_make "sz" (array_make "sz" "v").
 
   Definition dynarray_init : val :=
     λ: "sz" "fn",
-      assume (#0 ≤ "sz") ;;
-      record2_make "sz" (array_init "sz" (λ: "i", &Some (ref ("fn" "i")))).
+      record2_make "sz" (array_init "sz" "fn").
 
   Definition dynarray_size : val :=
     λ: "t",
       !"t".[size].
-  #[local] Definition dynarray_data : val :=
-    λ: "t",
-      !"t".[data].
-
-  #[local] Definition dynarray_set_size : val :=
-    λ: "t" "sz",
-      "t".[size] <- "sz".
-  #[local] Definition dynarray_set_data : val :=
-    λ: "t" "data",
-      "t".[data] <- "data".
 
   Definition dynarray_is_empty : val :=
     λ: "t",
@@ -72,85 +54,50 @@ Section heapGS.
 
   Definition dynarray_get : val :=
     λ: "t" "i",
-      match: array_get (dynarray_data "t") "i" with
-      | None =>
-          diverge #()
-      | Some "ref" =>
-          !"ref"
-      end.
+      array_get !"t".[data] "i".
 
   Definition dynarray_set : val :=
     λ: "t" "i" "v",
-      match: array_get (dynarray_data "t") "i" with
-      | None =>
-          diverge #()
-      | Some "ref" =>
-          "ref" <- "v"
-      end.
+      array_set !"t".[data] "i" "v".
 
   #[local] Definition dynarray_next_capacity : val :=
     λ: "n",
       maximum #8 (if: "n" ≤ #512 then #2 * "n" else "n" + "n" `quot` #2).
   Definition dynarray_reserve : val :=
     λ: "t" "n",
-      let: "data" := dynarray_data "t" in
+      let: "data" := !"t".[data] in
       let: "cap" := array_size "data" in
       if: "n" ≤ "cap" then (
         #()
       ) else (
-        assume (#0 ≤ "n") ;;
         let: "new_cap" := maximum "n" (dynarray_next_capacity "cap") in
-        let: "new_data" := array_make "new_cap" &None in
-        array_blit "data" #0 "new_data" #0 (dynarray_size "t") ;;
-        dynarray_set_data "t" "new_data"
+        let: "new_data" := array_make "new_cap" #() in
+        array_blit "data" #0 "new_data" #0 !"t".[size] ;;
+        "t".[data] <- "new_data"
       ).
   Definition dynarray_reserve_extra : val :=
     λ: "t" "n",
       if: #0 ≤ "n" then (
-        dynarray_reserve "t" (dynarray_size "t" + "n")
+        dynarray_reserve "t" (!"t".[size] + "n")
       ) else (
         #()
       ).
 
-  #[local] Definition dynarray_try_push : val :=
-    λ: "t" "slot",
-      let: "sz" := dynarray_size "t" in
-      let: "data" := dynarray_data "t" in
-      if: array_size "data" ≤ "sz" then (
-        #false
-      ) else (
-        array_unsafe_set "data" "sz" "slot" ;;
-        dynarray_set_size "t" ("sz" + #1) ;;
-        #true
-      ).
-  #[local] Definition dynarray_push_aux : val :=
-    rec: "dynarray_push_aux" "t" "slot" :=
-      dynarray_reserve_extra "t" #1 ;;
-      if: dynarray_try_push "t" "slot" then (
-        #()
-      ) else (
-        "dynarray_push_aux" "t" "slot"
-      ).
   Definition dynarray_push : val :=
     λ: "t" "v",
-      let: "slot" := &Some (ref "v") in
-      if: dynarray_try_push "t" "slot" then (
-        #()
-      ) else (
-        dynarray_push_aux "t" "slot"
-      ).
+      dynarray_reserve_extra "t" #1 ;;
+      let: "sz" := !"t".[size] in
+      "t".[size] <- "sz" + #1 ;;
+      array_set !"t".[data] "sz" "v".
 
   Section dynarray_model.
-    #[local] Definition slot_model slot v : iProp Σ :=
-      ∃ r,
-      ⌜slot = &&Some #r⌝ ∗
-      r ↦ v.
+    #[local] Definition dynarray_model_inner l (sz : nat) data vs : iProp Σ :=
+      l.[size] ↦ #sz ∗
+      l.[data] ↦ data ∗ array_model data (DfracOwn 1) vs.
     Definition dynarray_model t vs : iProp Σ :=
-      ∃ l data slots extra,
+      ∃ l data extra,
       ⌜t = #l⌝ ∗
-      l.[size] ↦ #(length vs) ∗
-      l.[data] ↦ data ∗ array_model data (DfracOwn 1) (slots ++ replicate extra &&None) ∗
-      [∗list] slot; v ∈ slots; vs, slot_model slot v.
+      dynarray_model_inner l (length vs) data (vs ++ replicate extra #()).
 
     #[global] Instance dynarray_model_timeless t vs :
       Timeless (dynarray_model t vs).
@@ -172,7 +119,7 @@ Section heapGS.
     wp_apply (array_create_spec with "[//]"). iIntros "%data Hdata_model".
     wp_apply (record2_make_spec with "[//]"). iIntros "%l (Hl & _)".
     iDestruct (record2_model_eq_1 with "Hl") as "(Hsz & Hdata)".
-    iApply "HΦ". iExists l, data, [], 0. iSmash.
+    iApply "HΦ". iExists l, data, 0. iSmash.
   Qed.
 
   Lemma dynarray_make_spec sz v :
@@ -187,13 +134,11 @@ Section heapGS.
     iIntros "% %Φ _ HΦ".
     Z_to_nat sz. rewrite Nat2Z.id.
     wp_rec.
-    wp_smart_apply assume_spec'. iIntros "_".
-    wp_smart_apply (array_init_spec_disentangled' (λ _ slot, slot_model slot v)); [done | iSmash |]. iIntros "%data %slots (%Hslots & Hdata_model & Hslots)".
+    wp_smart_apply (array_make_spec with "[//]"); first done. iIntros "%data Hdata_model".
     wp_apply (record2_make_spec with "[//]"). iIntros "%l (Hl & _)".
     iDestruct (record2_model_eq_1 with "Hl") as "(Hsz & Hdata)".
-    iApply "HΦ". iExists l, data, slots, 0. iFrame. iSplit; first iSmash.
-    rewrite replicate_length right_id. iFrame.
-    iApply (big_sepL2_replicate_r_2 _ _ (λ _, slot_model) with "Hslots"). lia.
+    iApply "HΦ". iExists l, data, 0. iFrame. iSplit; first iSmash.
+    rewrite replicate_length right_id Nat2Z.id. iSmash.
   Qed.
 
   Lemma dynarray_init_spec Ψ sz fn :
@@ -215,26 +160,11 @@ Section heapGS.
   Proof.
     iIntros "%Hsz %Φ (HΨ & Hfn) HΦ".
     wp_rec.
-    wp_smart_apply assume_spec'. iIntros "_".
-    pose Ψ' slots := (
-      ∃ vs,
-      Ψ vs ∗
-      [∗list] slot; v ∈ slots; vs, slot_model slot v
-    )%I.
-    wp_smart_apply (array_init_spec Ψ' with "[HΨ Hfn]"); first done.
-    { iSplitL "HΨ"; first iSmash.
-      iApply (big_sepL_impl with "Hfn"). iIntros "!> %i %_i %Hi Hfn %slots -> (%vs & HΨ & Hslots)".
-      iDestruct (big_sepL2_length with "Hslots") as %->.
-      wp_smart_apply (wp_wand with "(Hfn [//] HΨ)"). iIntros "%v HΨ".
-      wp_alloc r as "Hr". wp_pures.
-      iExists (vs ++ [v]). iFrame. iSmash.
-    }
-    iIntros "%data %slots (%Hslots & Hdata_model & (%vs & HΨ & Hslots))".
+    wp_smart_apply (array_init_spec Ψ with "[HΨ Hfn]"); [done | iSmash |]. iIntros "%data %vs (%Hvs & Hdata_model & HΨ)".
     wp_apply (record2_make_spec with "[//]"). iIntros "%l (Hl & _)".
     iDestruct (record2_model_eq_1 with "Hl") as "(Hsz & Hdata)".
-    iDestruct (big_sepL2_length with "Hslots") as %Hslots'.
     iApply "HΦ". iFrame. iSplit; first iSmash.
-    iExists l, data, slots, 0. iFrame. iSplitR; first iSmash. iSplitL "Hsz"; first iSmash.
+    iExists l, data, 0. iFrame. iSplitR; first iSmash. iSplitL "Hsz"; first iSmash.
     rewrite right_id //.
   Qed.
   Lemma dynarray_init_spec' Ψ sz fn :
@@ -346,15 +276,10 @@ Section heapGS.
       dynarray_model t vs
     }}}.
   Proof.
-    iIntros "%Hi %Hvs_lookup %Φ (%l & %data & %slots & %extra & -> & Hsz & Hdata & Hdata_model & Hslots) HΦ".
-    Z_to_nat i. rewrite Nat2Z.id in Hvs_lookup.
-    clear Hi. pose proof Hvs_lookup as Hi%lookup_lt_Some.
-    iDestruct (big_sepL2_length with "Hslots") as "%Hslots".
-    destruct (lookup_lt_is_Some_2 slots i) as (slot & Hslots_lookup); first lia.
-    iDestruct (big_sepL2_lookup_acc with "Hslots") as "((%r & %Hr & Hr) & Hslots)"; [done.. | subst slot].
-    wp_rec. rewrite /dynarray_data. wp_load.
-    wp_smart_apply (array_get_spec with "Hdata_model"); first lia.
-    { rewrite Nat2Z.id lookup_app_l //. lia. }
+    iIntros "%Hi %Hlookup %Φ (%l & %data & %extra & -> & Hsz & Hdata & Hdata_model) HΦ".
+    wp_rec. wp_load.
+    wp_apply (array_get_spec with "Hdata_model"); first done.
+    { rewrite lookup_app_l //. eapply lookup_lt_Some. done. }
     iSmash.
   Qed.
 
@@ -369,21 +294,13 @@ Section heapGS.
       dynarray_model t (<[Z.to_nat i := v]> vs)
     }}}.
   Proof.
-    iIntros "%Hi %Φ (%l & %data & %slots & %extra & -> & Hsz & Hdata & Hdata_model & Hslots) HΦ".
-    Z_to_nat i. rewrite Nat2Z.id.
-    iDestruct (big_sepL2_length with "Hslots") as "%Hslots".
-    feed pose proof (lookup_lookup_total vs i) as Hvs_lookup.
-    { apply lookup_lt_is_Some_2. lia. }
-    destruct (lookup_lt_is_Some_2 slots i) as (slot & Hslots_lookup); first lia.
-    iDestruct (big_sepL2_insert_acc with "Hslots") as "((%r & %Hr & Hr) & Hslots)"; [done.. | subst slot].
-    wp_rec. rewrite /dynarray_data. wp_load.
-    wp_smart_apply (array_get_spec with "Hdata_model"); first lia.
-    { rewrite Nat2Z.id lookup_app_l //. lia. }
+    iIntros "%Hi %Φ (%l & %data & %extra & -> & Hsz & Hdata & Hdata_model) HΦ".
+    wp_rec. wp_load.
+    wp_apply (array_set_spec with "Hdata_model").
+    { rewrite app_length replicate_length. lia. }
     iIntros "Hdata_model".
-    wp_store.
-    iDestruct ("Hslots" with "[Hr]") as "Hslots"; first iSmash.
-    rewrite (list_insert_id slots) //.
-    iApply "HΦ". iExists l, data, slots, extra. rewrite insert_length. iSmash.
+    iApply "HΦ". iExists l, data, extra.
+    rewrite insert_length insert_app_l; last lia. iSmash.
   Qed.
 
   #[local] Lemma dynarray_next_capacity_spec n :
@@ -398,6 +315,37 @@ Section heapGS.
     Ltac Zify.zify_post_hook ::= Z.quot_rem_to_equations.
     iSmash.
   Qed.
+  #[local] Lemma dynarray_reserve_spec' l data vs extra n :
+    (0 ≤ n)%Z →
+    {{{
+      dynarray_model_inner l (length vs) data (vs ++ replicate extra #())
+    }}}
+      dynarray_reserve #l #n
+    {{{ data' δ,
+      RET #();
+      ⌜Z.to_nat n ≤ length vs + δ⌝ ∗
+      dynarray_model_inner l (length vs) data' (vs ++ replicate δ #())
+    }}}.
+  Proof.
+    iIntros "%Hn %Φ (Hsz & Hdata & Hdata_model) HΦ".
+    wp_rec. wp_load.
+    wp_smart_apply (array_size_spec with "Hdata_model"). iIntros "Hdata_model".
+    wp_pures.
+    case_bool_decide as Htest; wp_pures; rewrite app_length replicate_length in Htest.
+    - iApply ("HΦ" $! data extra). iSmash.
+    - wp_apply (dynarray_next_capacity_spec with "[//]"); first lia. iIntros "%n' %Hn'".
+      rewrite app_length replicate_length in Hn'.
+      wp_apply maximum_spec.
+      wp_smart_apply (array_make_spec with "[//]"); first lia. iIntros "%data' Hdata_model'".
+      wp_load.
+      wp_smart_apply (array_blit_spec with "[$Hdata_model $Hdata_model']"); try lia.
+      { rewrite app_length replicate_length. lia. }
+      { rewrite replicate_length. lia. }
+      iIntros "(Hdata_model & Hdata_model')".
+      wp_store.
+      iApply ("HΦ" $! data' (Z.to_nat (n `max` n') - length vs)). iSplitR; first iSmash. iFrame.
+      rewrite Nat2Z.id drop_replicate take_app //.
+  Qed.
   Lemma dynarray_reserve_spec t vs n :
     (0 ≤ n)%Z →
     {{{
@@ -409,24 +357,28 @@ Section heapGS.
       dynarray_model t vs
     }}}.
   Proof.
-    iIntros "%Hn %Φ (%l & %data & %slots & %extra & -> & Hsz & Hdata & Hdata_model & Hslots) HΦ".
-    wp_rec. rewrite /dynarray_data. wp_load.
-    wp_smart_apply (array_size_spec with "Hdata_model"). iIntros "Hdata_model".
-    wp_pures.
-    case_bool_decide; wp_pures; first iSmash.
-    wp_smart_apply assume_spec'. iIntros "_".
-    wp_smart_apply (dynarray_next_capacity_spec with "[//]"); first lia. iIntros "%n' %Hn'".
-    wp_apply maximum_spec.
-    wp_smart_apply (array_make_spec with "[//]"); first lia. iIntros "%data' Hdata_model'".
-    rewrite /dynarray_size. wp_load.
-    iDestruct (big_sepL2_length with "Hslots") as "%Hslots".
-    wp_smart_apply (array_blit_spec with "[$Hdata_model $Hdata_model']"); try lia.
-    { rewrite app_length. lia. }
-    { rewrite replicate_length. rewrite app_length in Hn'. lia. }
-    iIntros "(Hdata_model & Hdata_model')".
-    rewrite /dynarray_set_data. wp_store.
-    iApply "HΦ". iExists l, data', slots, _. iFrame. iSplitR; first iSmash.
-    rewrite !Nat2Z.id drop_replicate take_app_alt //.
+    iIntros "%Hn %Φ (%l & %data & %extra & -> & Hmodel) HΦ".
+    wp_apply (dynarray_reserve_spec' with "Hmodel"); first done. iIntros "%data' %δ (%Hδ & Hmodel)".
+    iSmash.
+  Qed.
+  #[local] Lemma dynarray_reserve_extra_spec' l data vs extra n :
+    (0 ≤ n)%Z →
+    {{{
+      dynarray_model_inner l (length vs) data (vs ++ replicate extra #())
+    }}}
+      dynarray_reserve_extra #l #n
+    {{{ data' δ,
+      RET #();
+      ⌜Z.to_nat n ≤ δ⌝ ∗
+      dynarray_model_inner l (length vs) data' (vs ++ replicate δ #())
+    }}}.
+  Proof.
+    iIntros "%Hn %Φ (Hsz & Hdata & Hdata_model) HΦ".
+    wp_rec. wp_pures.
+    case_bool_decide; wp_pures; last iSmash.
+    wp_load.
+    wp_smart_apply (dynarray_reserve_spec' with "[Hsz Hdata Hdata_model]"); [lia | iSmash |]. iIntros "%data' %δ (%Hδ & Hmodel)".
+    iApply ("HΦ" $! data' δ). iSmash.
   Qed.
   Lemma dynarray_reserve_extra_spec t vs n :
     (0 ≤ n)%Z →
@@ -439,63 +391,11 @@ Section heapGS.
       dynarray_model t vs
     }}}.
   Proof.
-    iIntros "%Hn %Φ Hmodel HΦ".
-    wp_rec. wp_pures.
-    case_bool_decide; wp_pures; last iSmash+.
-    wp_apply (dynarray_size_spec with "Hmodel"). iIntros "Hmodel".
-    wp_smart_apply (dynarray_reserve_spec with "Hmodel"); first lia.
+    iIntros "%Hn %Φ (%l & %data & %extra & -> & Hmodel) HΦ".
+    wp_apply (dynarray_reserve_extra_spec' with "Hmodel"); first done. iIntros "%data' %δ (%Hδ & Hmodel)".
     iSmash.
   Qed.
 
-  #[local] Lemma dynarray_try_push_spec t vs slot v :
-    {{{
-      dynarray_model t vs ∗
-      slot_model slot v
-    }}}
-      dynarray_try_push t slot
-    {{{ b,
-      RET #b;
-      if b then
-        dynarray_model t (vs ++ [v])
-      else
-        dynarray_model t vs ∗
-        slot_model slot v
-    }}}.
-  Proof.
-    iIntros "%Φ ((%l & %data & %slots & %extra & -> & Hsz & Hdata & Hdata_model & Hslots) & Hslot) HΦ".
-    iDestruct (big_sepL2_length with "Hslots") as "%Hslots".
-    wp_rec. rewrite /dynarray_size /dynarray_data. do 2 wp_load.
-    wp_smart_apply (array_size_spec with "Hdata_model"). iIntros "Hdata_model".
-    wp_pures.
-    case_bool_decide as Htest; wp_pures.
-    { iApply "HΦ". iFrame. iSmash. }
-    wp_apply (array_unsafe_set_spec with "Hdata_model"); first lia. iIntros "Hdata_model".
-    rewrite /dynarray_set_size. wp_store.
-    iApply "HΦ". iExists l, data, (slots ++ [slot]), (extra - 1). iFrame. iSplitR; first iSmash.
-    rewrite app_length Z.add_1_r -Nat2Z.inj_succ Nat.add_comm /=. iFrame.
-    rewrite Nat2Z.id -Hslots -(Nat.add_0_r (length slots)) insert_app_r.
-    destruct extra.
-    - rewrite app_length in Htest. naive_solver lia.
-    - rewrite -(assoc (++)) /= Nat.sub_0_r. iSmash.
-  Qed.
-  #[local] Lemma dynarray_push_aux_spec t vs slot v :
-    {{{
-      dynarray_model t vs ∗
-      slot_model slot v
-    }}}
-      dynarray_push_aux t slot
-    {{{
-      RET #();
-      dynarray_model t (vs ++ [v])
-    }}}.
-  Proof.
-    iIntros "%Φ (Hmodel & Hslot) HΦ".
-    iLöb as "HLöb".
-    wp_rec.
-    wp_smart_apply (dynarray_reserve_extra_spec with "Hmodel"); first lia. iIntros "Hmodel".
-    wp_smart_apply (dynarray_try_push_spec with "[$Hmodel $Hslot]"). iIntros ([]); first iSmash. iIntros "(Hmodel & Hslot)".
-    wp_smart_apply ("HLöb" with "Hmodel Hslot HΦ").
-  Qed.
   Lemma dynarray_push_spec t vs v :
     {{{
       dynarray_model t vs
@@ -506,266 +406,14 @@ Section heapGS.
       dynarray_model t (vs ++ [v])
     }}}.
   Proof.
-    iIntros "%Φ Hmodel HΦ".
-    wp_rec. wp_alloc r as "Hr".
-    wp_smart_apply (dynarray_try_push_spec with "[$Hmodel Hr]"); first iSmash. iIntros ([]); first iSmash. iIntros "(Hmodel & Hslot)".
-    wp_smart_apply (dynarray_push_aux_spec with "[$Hmodel $Hslot]").
-    iSmash.
-  Qed.
-
-  Context τ `{!iType (iPropI Σ) τ}.
-
-  #[local] Definition slot_type :=
-    opt_type (reference_type τ).
-  Definition dynarray_type t : iProp Σ :=
-    ∃ l,
-    ⌜t = #l⌝ ∗
-    inv nroot (
-      ∃ (sz : nat) cap data,
-      l.[size] ↦ #sz ∗
-      l.[data] ↦ data ∗ array_type slot_type cap data
-    ).
-  #[global] Instance dynarray_type_itype :
-    iType _ dynarray_type.
-  Proof.
-    split. apply _.
-  Qed.
-
-  Lemma dynarray_create_type :
-    {{{ True }}}
-      dynarray_create #()
-    {{{ t,
-      RET t;
-      dynarray_type t
-    }}}.
-  Proof.
-    iIntros "%Φ _ HΦ".
+    iIntros "%Φ (%l & %data & %extra & -> & Hmodel) HΦ".
     wp_rec.
-    wp_apply (array_create_type slot_type with "[//]"). iIntros "%data Hdata_type".
-    iApply wp_fupd.
-    wp_apply (record2_make_spec with "[//]"). iIntros "%l (Hl & _)". iDestruct (record2_model_eq_1 with "Hl") as "(Hsz & Hdata)".
-    iSmash.
-  Qed.
-
-  Lemma dynarray_make_type sz v :
-    {{{
-      int_type sz ∗
-      τ v
-    }}}
-      dynarray_make sz v
-    {{{ t,
-      RET t;
-      dynarray_type t
-    }}}.
-  Proof.
-    iIntros "%Φ ((%sz_ & ->) & #Hv) HΦ".
-    wp_rec.
-    wp_smart_apply assume_spec'. iIntros "%Hsz".
-    Z_to_nat sz_ as sz.
-    wp_smart_apply (array_init_type slot_type); first iSmash. iIntros "%data Hdata_type".
-    iApply wp_fupd.
-    wp_smart_apply (record2_make_spec with "[//]"). iIntros "%l (Hl & _)". iDestruct (record2_model_eq_1 with "Hl") as "(Hsz & Hdata)".
-    iSmash.
-  Qed.
-
-  Lemma dynarray_size_type t :
-    {{{
-      dynarray_type t
-    }}}
-      dynarray_size t
-    {{{ (sz : nat),
-      RET #sz; True
-    }}}.
-  Proof.
-    iSmash.
-  Qed.
-
-  #[local] Lemma dynarray_data_type t :
-    {{{
-      dynarray_type t
-    }}}
-      dynarray_data t
-    {{{ cap data,
-      RET data;
-      array_type slot_type cap data
-    }}}.
-  Proof.
-    iSmash.
-  Qed.
-
-  #[local] Lemma dynarray_set_size_type t sz :
-    {{{
-      dynarray_type t ∗
-      nat_type sz
-    }}}
-      dynarray_set_size t sz
-    {{{
-      RET #(); True
-    }}}.
-  Proof.
-    iSmash.
-  Qed.
-
-  #[local] Lemma dynarray_set_data_type t cap data :
-    {{{
-      dynarray_type t ∗
-      array_type slot_type cap data
-    }}}
-      dynarray_set_data t data
-    {{{
-      RET #(); True
-    }}}.
-  Proof.
-    iSmash.
-  Qed.
-
-  Lemma dynarray_is_empty_type t :
-    {{{
-      dynarray_type t
-    }}}
-      dynarray_is_empty t
-    {{{ b,
-      RET #b; True
-    }}}.
-  Proof.
-    iSmash.
-  Qed.
-
-  Lemma dynarray_get_type t (i : val) :
-    {{{
-      dynarray_type t ∗
-      int_type i
-    }}}
-      dynarray_get t i
-    {{{ v,
-      RET v;
-      τ v
-    }}}.
-  Proof.
-    iIntros "%Φ (#Htype & (%i_ & ->)) HΦ".
-    wp_rec.
-    wp_smart_apply (dynarray_data_type with "Htype"). iIntros "%cap %data #Hdata_type".
-    wp_apply (array_get_type with "[$Hdata_type]"); first iSmash. iIntros "%v [-> | (%ref & -> & #Href)]".
-    - wp_smart_apply wp_diverge.
-    - wp_smart_apply (reference_get_type with "Href"). iSmash.
-  Qed.
-
-  Lemma dynarray_set_type t (i : val) v :
-    {{{
-      dynarray_type t ∗
-      int_type i ∗
-      τ v
-    }}}
-      dynarray_set t i v
-    {{{
-      RET #(); True
-    }}}.
-  Proof.
-    iIntros "%Φ (#Htype & (%i_ & ->) & #Hv) HΦ".
-    wp_rec.
-    wp_smart_apply (dynarray_data_type with "Htype"). iIntros "%cap %data #Hdata_type".
-    wp_apply (array_get_type with "[$Hdata_type]"); first iSmash. iIntros "%w [-> | (%ref & -> & #Href)]".
-    - wp_smart_apply wp_diverge.
-    - wp_smart_apply (reference_set_type with "[$Href $Hv]"). iSmash.
-  Qed.
-
-  Lemma dynarray_reserve_type t n :
-    {{{
-      dynarray_type t ∗
-      int_type n
-    }}}
-      dynarray_reserve t n
-    {{{
-      RET #(); True
-    }}}.
-  Proof.
-    iIntros "%Φ (#Htype & (%n_ & ->)) HΦ".
-    wp_rec.
-    wp_smart_apply (dynarray_data_type with "Htype"). iIntros "%cap %data #Hdata_type".
-    wp_smart_apply (array_size_type with "Hdata_type"). iIntros "_".
-    wp_pures.
-    case_bool_decide; wp_pures; first iSmash.
-    wp_apply assume_spec'. iIntros "%Hn".
-    wp_smart_apply (dynarray_next_capacity_spec with "[//]"); first lia. iIntros "%n' %Hn'".
-    wp_apply maximum_spec.
-    wp_smart_apply (array_make_type slot_type); first iSmash. iIntros "%data' #Hdata_type'".
-    wp_smart_apply dynarray_size_type; first iSmash+. iIntros "%sz _".
-    wp_smart_apply (array_blit_type slot_type); first iSmash. iIntros "_".
-    wp_smart_apply (dynarray_set_data_type with "[$Htype $Hdata_type']"). iIntros "_".
-    iSmash.
-  Qed.
-  Lemma dynarray_reserve_extra_type t n :
-    {{{
-      dynarray_type t ∗
-      int_type n
-    }}}
-      dynarray_reserve_extra t n
-    {{{
-      RET #(); True
-    }}}.
-  Proof.
-    iIntros "%Φ (#Htype & (%n_ & ->)) HΦ".
-    wp_rec. wp_pures.
-    case_bool_decide; wp_pures; last iSmash.
-    wp_apply (dynarray_size_type with "Htype"). iIntros "%sz _".
-    wp_smart_apply (dynarray_reserve_type with "[$Htype]"); first iSmash.
-    iSmash.
-  Qed.
-
-  #[local] Lemma dynarray_try_push_type t slot :
-    {{{
-      dynarray_type t ∗
-      slot_type slot
-    }}}
-      dynarray_try_push t slot
-    {{{ b,
-      RET #b; True
-    }}}.
-  Proof.
-    iIntros "%Φ (#Htype & #Hslot) HΦ".
-    wp_rec.
-    wp_smart_apply (dynarray_size_type with "Htype"). iIntros "%sz _".
-    wp_smart_apply (dynarray_data_type with "Htype"). iIntros "%cap %data #Hdata_type".
-    wp_smart_apply (array_size_type with "Hdata_type"). iIntros "_".
-    wp_pures.
-    case_bool_decide; wp_pures; first iSmash.
-    wp_apply (array_unsafe_set_type with "[$Hdata_type $Hslot]"); first lia. iIntros "_".
-    wp_smart_apply (dynarray_set_size_type with "[$Htype]"); first iSmash. iIntros "_".
-    iSmash.
-  Qed.
-  #[local] Lemma dynarray_push_aux_type t slot :
-    {{{
-      dynarray_type t ∗
-      slot_type slot
-    }}}
-      dynarray_push_aux t slot
-    {{{
-      RET #(); True
-    }}}.
-  Proof.
-    iIntros "%Φ (#Htype & #Hslot) HΦ".
-    iLöb as "HLöb".
-    wp_rec.
-    wp_smart_apply (dynarray_reserve_extra_type with "[$Htype]"); first iSmash. iIntros "_".
-    wp_smart_apply (dynarray_try_push_type with "[$Htype $Hslot]"). iIntros ([]) "_"; first iSmash.
-    wp_smart_apply ("HLöb" with "HΦ").
-  Qed.
-  Lemma dynarray_push_type t v :
-    {{{
-      dynarray_type t ∗
-      τ v
-    }}}
-      dynarray_push t v
-    {{{
-      RET #(); True
-    }}}.
-  Proof.
-    iIntros "%Φ (#Htype & #Hv) HΦ".
-    wp_rec. wp_alloc r as "Hr".
-    iAssert (|={⊤}=> slot_type (&&Some #r))%I with "[Hr]" as ">#Hslot"; first iSmash.
-    wp_smart_apply (dynarray_try_push_type with "[$Htype $Hslot]"). iIntros ([]) "_"; first iSmash.
-    wp_smart_apply (dynarray_push_aux_type with "[$Htype $Hslot]"). iIntros "_".
-    iSmash.
+    wp_smart_apply (dynarray_reserve_extra_spec' with "Hmodel"); first lia. iIntros "%data' %δ (%Hδ & (Hsz & Hdata & Hdata_model))".
+    wp_load. wp_store. wp_load.
+    wp_apply (array_set_spec with "Hdata_model").
+    { rewrite app_length replicate_length. lia. }
+    rewrite Nat2Z.id insert_app_r_alt // Nat.sub_diag insert_replicate_lt // /= (assoc (++) vs [v] (replicate _ _)).
+    iSteps. rewrite app_length. iSmash.
   Qed.
 End heapGS.
 
@@ -781,4 +429,3 @@ End heapGS.
 #[global] Opaque dynarray_push.
 
 #[global] Opaque dynarray_model.
-#[global] Opaque dynarray_type.
