theories/std/safe_dynarray.v
@@ -1,0 +1,784 @@
+From ml Require Import
+  prelude.
+From ml.bi Require Import
+  big_op.
+From ml.language Require Import
+  notations
+  proofmode.
+From ml.std Require Export
+  base.
+From ml.std Require Import
+  diverge
+  assume
+  record2
+  math
+  reference
+  opt
+  array.
+
+Section heapGS.
+  Context `{!heapGS Σ}.
+
+  Implicit Types b : bool.
+  Implicit Types i : nat.
+  Implicit Types l r : loc.
+  Implicit Types v t fn : val.
+  Implicit Types vs : list val.
+
+  Notation "t '.[size]'" := t.[0]%stdpp
+  ( at level 5
+  ) : stdpp_scope.
+  Notation "t '.[data]'" := t.[1]%stdpp
+  ( at level 5
+  ) : stdpp_scope.
+  Notation "t '.[size]'" := t.[0]%E
+  ( at level 5
+  ) : expr_scope.
+  Notation "t '.[data]'" := t.[1]%E
+  ( at level 5
+  ) : expr_scope.
+
+  Definition safe_dynarray_create : val :=
+    λ: <>,
+      record2_make #0 (array_create #()).
+
+  Definition safe_dynarray_make : val :=
+    λ: "sz" "v",
+      assume (#0 ≤ "sz") ;;
+      record2_make "sz" (array_init "sz" (λ: <>, &Some (ref "v"))).
+
+  Definition safe_dynarray_init : val :=
+    λ: "sz" "fn",
+      assume (#0 ≤ "sz") ;;
+      record2_make "sz" (array_init "sz" (λ: "i", &Some (ref ("fn" "i")))).
+
+  Definition safe_dynarray_size : val :=
+    λ: "t",
+      !"t".[size].
+  #[local] Definition safe_dynarray_data : val :=
+    λ: "t",
+      !"t".[data].
+
+  #[local] Definition safe_dynarray_set_size : val :=
+    λ: "t" "sz",
+      "t".[size] <- "sz".
+  #[local] Definition safe_dynarray_set_data : val :=
+    λ: "t" "data",
+      "t".[data] <- "data".
+
+  Definition safe_dynarray_is_empty : val :=
+    λ: "t",
+      safe_dynarray_size "t" = #0.
+
+  Definition safe_dynarray_get : val :=
+    λ: "t" "i",
+      match: array_get (safe_dynarray_data "t") "i" with
+      | None =>
+          diverge #()
+      | Some "ref" =>
+          !"ref"
+      end.
+
+  Definition safe_dynarray_set : val :=
+    λ: "t" "i" "v",
+      match: array_get (safe_dynarray_data "t") "i" with
+      | None =>
+          diverge #()
+      | Some "ref" =>
+          "ref" <- "v"
+      end.
+
+  #[local] Definition safe_dynarray_next_capacity : val :=
+    λ: "n",
+      maximum #8 (if: "n" ≤ #512 then #2 * "n" else "n" + "n" `quot` #2).
+  Definition safe_dynarray_reserve : val :=
+    λ: "t" "n",
+      let: "data" := safe_dynarray_data "t" in
+      let: "cap" := array_size "data" in
+      if: "n" ≤ "cap" then (
+        #()
+      ) else (
+        assume (#0 ≤ "n") ;;
+        let: "new_cap" := maximum "n" (safe_dynarray_next_capacity "cap") in
+        let: "new_data" := array_make "new_cap" &None in
+        array_blit "data" #0 "new_data" #0 (safe_dynarray_size "t") ;;
+        safe_dynarray_set_data "t" "new_data"
+      ).
+  Definition safe_dynarray_reserve_extra : val :=
+    λ: "t" "n",
+      if: #0 ≤ "n" then (
+        safe_dynarray_reserve "t" (safe_dynarray_size "t" + "n")
+      ) else (
+        #()
+      ).
+
+  #[local] Definition safe_dynarray_try_push : val :=
+    λ: "t" "slot",
+      let: "sz" := safe_dynarray_size "t" in
+      let: "data" := safe_dynarray_data "t" in
+      if: array_size "data" ≤ "sz" then (
+        #false
+      ) else (
+        array_unsafe_set "data" "sz" "slot" ;;
+        safe_dynarray_set_size "t" ("sz" + #1) ;;
+        #true
+      ).
+  #[local] Definition safe_dynarray_push_aux : val :=
+    rec: "safe_dynarray_push_aux" "t" "slot" :=
+      safe_dynarray_reserve_extra "t" #1 ;;
+      if: safe_dynarray_try_push "t" "slot" then (
+        #()
+      ) else (
+        "safe_dynarray_push_aux" "t" "slot"
+      ).
+  Definition safe_dynarray_push : val :=
+    λ: "t" "v",
+      let: "slot" := &Some (ref "v") in
+      if: safe_dynarray_try_push "t" "slot" then (
+        #()
+      ) else (
+        safe_dynarray_push_aux "t" "slot"
+      ).
+
+  Section safe_dynarray_model.
+    #[local] Definition slot_model slot v : iProp Σ :=
+      ∃ r,
+      ⌜slot = &&Some #r⌝ ∗
+      r ↦ v.
+    Definition safe_dynarray_model t vs : iProp Σ :=
+      ∃ l data slots extra,
+      ⌜t = #l⌝ ∗
+      l.[size] ↦ #(length vs) ∗
+      l.[data] ↦ data ∗ array_model data (DfracOwn 1) (slots ++ replicate extra &&None) ∗
+      [∗list] slot; v ∈ slots; vs, slot_model slot v.
+
+    #[global] Instance safe_dynarray_model_timeless t vs :
+      Timeless (safe_dynarray_model t vs).
+    Proof.
+      apply _.
+    Qed.
+  End safe_dynarray_model.
+
+  Lemma safe_dynarray_create_spec :
+    {{{ True }}}
+      safe_dynarray_create #()
+    {{{ t,
+      RET t;
+      safe_dynarray_model t []
+    }}}.
+  Proof.
+    iIntros "%Φ _ HΦ".
+    wp_rec.
+    wp_apply (array_create_spec with "[//]"). iIntros "%data Hdata_model".
+    wp_apply (record2_make_spec with "[//]"). iIntros "%l (Hl & _)".
+    iDestruct (record2_model_eq_1 with "Hl") as "(Hsz & Hdata)".
+    iApply "HΦ". iExists l, data, [], 0. iSmash.
+  Qed.
+
+  Lemma safe_dynarray_make_spec sz v :
+    (0 ≤ sz)%Z →
+    {{{ True }}}
+      safe_dynarray_make #sz v
+    {{{ t,
+      RET t;
+      safe_dynarray_model t (replicate (Z.to_nat sz) v)
+    }}}.
+  Proof.
+    iIntros "% %Φ _ HΦ".
+    Z_to_nat sz. rewrite Nat2Z.id.
+    wp_rec.
+    wp_smart_apply assume_spec'. iIntros "_".
+    wp_smart_apply (array_init_spec_disentangled' (λ _ slot, slot_model slot v)); [done | iSmash |]. iIntros "%data %slots (%Hslots & Hdata_model & Hslots)".
+    wp_apply (record2_make_spec with "[//]"). iIntros "%l (Hl & _)".
+    iDestruct (record2_model_eq_1 with "Hl") as "(Hsz & Hdata)".
+    iApply "HΦ". iExists l, data, slots, 0. iFrame. iSplit; first iSmash.
+    rewrite replicate_length right_id. iFrame.
+    iApply (big_sepL2_replicate_r_2 _ _ (λ _, slot_model) with "Hslots"). lia.
+  Qed.
+
+  Lemma safe_dynarray_init_spec Ψ sz fn :
+    (0 ≤ sz)%Z →
+    {{{
+      Ψ [] ∗
+      [∗ list] i ∈ seq 0 (Z.to_nat sz), ∀ vs_done,
+        ⌜i = length vs_done⌝ -∗
+        Ψ vs_done -∗
+        WP fn #(i : nat) {{ v, Ψ (vs_done ++ [v]) }}
+    }}}
+      safe_dynarray_init #sz fn
+    {{{ t vs,
+      RET t ;
+      ⌜length vs = Z.to_nat sz⌝ ∗
+      safe_dynarray_model t vs ∗
+      Ψ vs
+    }}}.
+  Proof.
+    iIntros "%Hsz %Φ (HΨ & Hfn) HΦ".
+    wp_rec.
+    wp_smart_apply assume_spec'. iIntros "_".
+    pose Ψ' slots := (
+      ∃ vs,
+      Ψ vs ∗
+      [∗list] slot; v ∈ slots; vs, slot_model slot v
+    )%I.
+    wp_smart_apply (array_init_spec Ψ' with "[HΨ Hfn]"); first done.
+    { iSplitL "HΨ"; first iSmash.
+      iApply (big_sepL_impl with "Hfn"). iIntros "!> %i %_i %Hi Hfn %slots -> (%vs & HΨ & Hslots)".
+      iDestruct (big_sepL2_length with "Hslots") as %->.
+      wp_smart_apply (wp_wand with "(Hfn [//] HΨ)"). iIntros "%v HΨ".
+      wp_alloc r as "Hr". wp_pures.
+      iExists (vs ++ [v]). iFrame. iSmash.
+    }
+    iIntros "%data %slots (%Hslots & Hdata_model & (%vs & HΨ & Hslots))".
+    wp_apply (record2_make_spec with "[//]"). iIntros "%l (Hl & _)".
+    iDestruct (record2_model_eq_1 with "Hl") as "(Hsz & Hdata)".
+    iDestruct (big_sepL2_length with "Hslots") as %Hslots'.
+    iApply "HΦ". iFrame. iSplit; first iSmash.
+    iExists l, data, slots, 0. iFrame. iSplitR; first iSmash. iSplitL "Hsz"; first iSmash.
+    rewrite right_id //.
+  Qed.
+  Lemma safe_dynarray_init_spec' Ψ sz fn :
+    (0 ≤ sz)%Z →
+    {{{
+      Ψ [] ∗
+      ∀ i vs_done,
+      {{{ ⌜i = length vs_done ∧ i < Z.to_nat sz⌝ ∗ Ψ vs_done }}}
+        fn #i
+      {{{ v, RET v; Ψ (vs_done ++ [v]) }}}
+    }}}
+      safe_dynarray_init #sz fn
+    {{{ t vs,
+      RET t ;
+      ⌜length vs = Z.to_nat sz⌝ ∗
+      safe_dynarray_model t vs ∗
+      Ψ vs
+    }}}.
+  Proof.
+    iIntros "% %Φ (HΨ & #Hfn) HΦ".
+    wp_apply (safe_dynarray_init_spec Ψ with "[$HΨ]"); try done.
+    iApply big_sepL_intro. iIntros "!> %i %_i %H_i %vs_done % HΨ". apply lookup_seq in H_i as (-> & ?).
+    iApply ("Hfn" with "[$HΨ]"); iSmash.
+  Qed.
+  Lemma safe_dynarray_init_spec_disentangled Ψ sz fn :
+    (0 ≤ sz)%Z →
+    {{{
+      [∗ list] i ∈ seq 0 (Z.to_nat sz),
+        WP fn #(i : nat) {{ Ψ i }}
+    }}}
+      safe_dynarray_init #sz fn
+    {{{ t vs,
+      RET t ;
+      ⌜length vs = Z.to_nat sz⌝ ∗
+      safe_dynarray_model t vs ∗
+      ([∗ list] i ↦ v ∈ vs, Ψ i v)
+    }}}.
+  Proof.
+    iIntros "% %Φ Hfn HΦ".
+    set (Ψ' vs := ([∗ list] i ↦ v ∈ vs, Ψ i v)%I).
+    wp_apply (safe_dynarray_init_spec Ψ' with "[Hfn]"); try done.
+    iSplit; first rewrite /Ψ' //.
+    iApply (big_sepL_mono with "Hfn"). iIntros "%i %v % Hfn %vs_done -> HΨ'".
+    iApply (wp_wand with "Hfn"). iIntros "%v HΨ". iFrame. iSplitL; last iSmash.
+    rewrite right_id //.
+  Qed.
+  Lemma safe_dynarray_init_spec_disentangled' Ψ sz fn :
+    (0 ≤ sz)%Z →
+    {{{
+      ∀ i,
+      {{{ ⌜i < Z.to_nat sz⌝ }}}
+        fn #i
+      {{{ v, RET v; Ψ i v }}}
+    }}}
+      safe_dynarray_init #sz fn
+    {{{ t vs,
+      RET t ;
+      ⌜length vs = Z.to_nat sz⌝ ∗
+      safe_dynarray_model t vs ∗
+      ([∗ list] i ↦ v ∈ vs, Ψ i v)
+    }}}.
+  Proof.
+    iIntros "% %Φ #Hfn HΦ".
+    wp_apply safe_dynarray_init_spec_disentangled; try done.
+    iApply  big_sepL_intro. iIntros "!> %i %_i %Hlookup".
+    apply lookup_seq in Hlookup as (-> & ?).
+    iApply ("Hfn" with "[//]"). iSmash.
+  Qed.
+
+  Lemma safe_dynarray_size_spec t vs :
+    {{{
+      safe_dynarray_model t vs
+    }}}
+      safe_dynarray_size t
+    {{{
+      RET #(length vs);
+      safe_dynarray_model t vs
+    }}}.
+  Proof.
+    iSmash.
+  Qed.
+
+  Lemma safe_dynarray_is_empty_spec t vs :
+    {{{
+      safe_dynarray_model t vs
+    }}}
+      safe_dynarray_is_empty t
+    {{{
+      RET #(bool_decide (vs = []));
+      safe_dynarray_model t vs
+    }}}.
+  Proof.
+    iIntros "%Φ Hmodel HΦ".
+    wp_rec.
+    wp_smart_apply (safe_dynarray_size_spec with "Hmodel"). iIntros "Hmodel".
+    wp_pures.
+    destruct vs; iApply ("HΦ" with "Hmodel").
+  Qed.
+
+  Lemma safe_dynarray_get_spec t vs (i : Z) v :
+    (0 ≤ i)%Z →
+    vs !! Z.to_nat i = Some v →
+    {{{
+      safe_dynarray_model t vs
+    }}}
+      safe_dynarray_get t #i
+    {{{
+      RET v;
+      safe_dynarray_model t vs
+    }}}.
+  Proof.
+    iIntros "%Hi %Hvs_lookup %Φ (%l & %data & %slots & %extra & -> & Hsz & Hdata & Hdata_model & Hslots) HΦ".
+    Z_to_nat i. rewrite Nat2Z.id in Hvs_lookup.
+    clear Hi. pose proof Hvs_lookup as Hi%lookup_lt_Some.
+    iDestruct (big_sepL2_length with "Hslots") as "%Hslots".
+    destruct (lookup_lt_is_Some_2 slots i) as (slot & Hslots_lookup); first lia.
+    iDestruct (big_sepL2_lookup_acc with "Hslots") as "((%r & %Hr & Hr) & Hslots)"; [done.. | subst slot].
+    wp_rec. rewrite /safe_dynarray_data. wp_load.
+    wp_smart_apply (array_get_spec with "Hdata_model"); first lia.
+    { rewrite Nat2Z.id lookup_app_l //. lia. }
+    iSmash.
+  Qed.
+
+  Lemma safe_dynarray_set_spec t vs (i : Z) v :
+    (0 ≤ i < length vs)%Z →
+    {{{
+      safe_dynarray_model t vs
+    }}}
+      safe_dynarray_set t #i v
+    {{{
+      RET #();
+      safe_dynarray_model t (<[Z.to_nat i := v]> vs)
+    }}}.
+  Proof.
+    iIntros "%Hi %Φ (%l & %data & %slots & %extra & -> & Hsz & Hdata & Hdata_model & Hslots) HΦ".
+    Z_to_nat i. rewrite Nat2Z.id.
+    iDestruct (big_sepL2_length with "Hslots") as "%Hslots".
+    feed pose proof (lookup_lookup_total vs i) as Hvs_lookup.
+    { apply lookup_lt_is_Some_2. lia. }
+    destruct (lookup_lt_is_Some_2 slots i) as (slot & Hslots_lookup); first lia.
+    iDestruct (big_sepL2_insert_acc with "Hslots") as "((%r & %Hr & Hr) & Hslots)"; [done.. | subst slot].
+    wp_rec. rewrite /safe_dynarray_data. wp_load.
+    wp_smart_apply (array_get_spec with "Hdata_model"); first lia.
+    { rewrite Nat2Z.id lookup_app_l //. lia. }
+    iIntros "Hdata_model".
+    wp_store.
+    iDestruct ("Hslots" with "[Hr]") as "Hslots"; first iSmash.
+    rewrite (list_insert_id slots) //.
+    iApply "HΦ". iExists l, data, slots, extra. rewrite insert_length. iSmash.
+  Qed.
+
+  #[local] Lemma safe_dynarray_next_capacity_spec n :
+    (0 ≤ n)%Z →
+    {{{ True }}}
+      safe_dynarray_next_capacity #n
+    {{{ m,
+      RET #m;
+      ⌜n ≤ m⌝%Z
+    }}}.
+  Proof.
+    Ltac Zify.zify_post_hook ::= Z.quot_rem_to_equations.
+    iSmash.
+  Qed.
+  Lemma safe_dynarray_reserve_spec t vs n :
+    (0 ≤ n)%Z →
+    {{{
+      safe_dynarray_model t vs
+    }}}
+      safe_dynarray_reserve t #n
+    {{{
+      RET #();
+      safe_dynarray_model t vs
+    }}}.
+  Proof.
+    iIntros "%Hn %Φ (%l & %data & %slots & %extra & -> & Hsz & Hdata & Hdata_model & Hslots) HΦ".
+    wp_rec. rewrite /safe_dynarray_data. wp_load.
+    wp_smart_apply (array_size_spec with "Hdata_model"). iIntros "Hdata_model".
+    wp_pures.
+    case_bool_decide; wp_pures; first iSmash.
+    wp_smart_apply assume_spec'. iIntros "_".
+    wp_smart_apply (safe_dynarray_next_capacity_spec with "[//]"); first lia. iIntros "%n' %Hn'".
+    wp_apply maximum_spec.
+    wp_smart_apply (array_make_spec with "[//]"); first lia. iIntros "%data' Hdata_model'".
+    rewrite /safe_dynarray_size. wp_load.
+    iDestruct (big_sepL2_length with "Hslots") as "%Hslots".
+    wp_smart_apply (array_blit_spec with "[$Hdata_model $Hdata_model']"); try lia.
+    { rewrite app_length. lia. }
+    { rewrite replicate_length. rewrite app_length in Hn'. lia. }
+    iIntros "(Hdata_model & Hdata_model')".
+    rewrite /safe_dynarray_set_data. wp_store.
+    iApply "HΦ". iExists l, data', slots, _. iFrame. iSplitR; first iSmash.
+    rewrite !Nat2Z.id drop_replicate take_app_alt //.
+  Qed.
+  Lemma safe_dynarray_reserve_extra_spec t vs n :
+    (0 ≤ n)%Z →
+    {{{
+      safe_dynarray_model t vs
+    }}}
+      safe_dynarray_reserve_extra t #n
+    {{{
+      RET #();
+      safe_dynarray_model t vs
+    }}}.
+  Proof.
+    iIntros "%Hn %Φ Hmodel HΦ".
+    wp_rec. wp_pures.
+    case_bool_decide; wp_pures; last iSmash+.
+    wp_apply (safe_dynarray_size_spec with "Hmodel"). iIntros "Hmodel".
+    wp_smart_apply (safe_dynarray_reserve_spec with "Hmodel"); first lia.
+    iSmash.
+  Qed.
+
+  #[local] Lemma safe_dynarray_try_push_spec t vs slot v :
+    {{{
+      safe_dynarray_model t vs ∗
+      slot_model slot v
+    }}}
+      safe_dynarray_try_push t slot
+    {{{ b,
+      RET #b;
+      if b then
+        safe_dynarray_model t (vs ++ [v])
+      else
+        safe_dynarray_model t vs ∗
+        slot_model slot v
+    }}}.
+  Proof.
+    iIntros "%Φ ((%l & %data & %slots & %extra & -> & Hsz & Hdata & Hdata_model & Hslots) & Hslot) HΦ".
+    iDestruct (big_sepL2_length with "Hslots") as "%Hslots".
+    wp_rec. rewrite /safe_dynarray_size /safe_dynarray_data. do 2 wp_load.
+    wp_smart_apply (array_size_spec with "Hdata_model"). iIntros "Hdata_model".
+    wp_pures.
+    case_bool_decide as Htest; wp_pures.
+    { iApply "HΦ". iFrame. iSmash. }
+    wp_apply (array_unsafe_set_spec with "Hdata_model"); first lia. iIntros "Hdata_model".
+    rewrite /safe_dynarray_set_size. wp_store.
+    iApply "HΦ". iExists l, data, (slots ++ [slot]), (extra - 1). iFrame. iSplitR; first iSmash.
+    rewrite app_length Z.add_1_r -Nat2Z.inj_succ Nat.add_comm /=. iFrame.
+    rewrite Nat2Z.id -Hslots -(Nat.add_0_r (length slots)) insert_app_r.
+    destruct extra.
+    - rewrite app_length in Htest. naive_solver lia.
+    - rewrite -(assoc (++)) /= Nat.sub_0_r. iSmash.
+  Qed.
+  #[local] Lemma safe_dynarray_push_aux_spec t vs slot v :
+    {{{
+      safe_dynarray_model t vs ∗
+      slot_model slot v
+    }}}
+      safe_dynarray_push_aux t slot
+    {{{
+      RET #();
+      safe_dynarray_model t (vs ++ [v])
+    }}}.
+  Proof.
+    iIntros "%Φ (Hmodel & Hslot) HΦ".
+    iLöb as "HLöb".
+    wp_rec.
+    wp_smart_apply (safe_dynarray_reserve_extra_spec with "Hmodel"); first lia. iIntros "Hmodel".
+    wp_smart_apply (safe_dynarray_try_push_spec with "[$Hmodel $Hslot]"). iIntros ([]); first iSmash. iIntros "(Hmodel & Hslot)".
+    wp_smart_apply ("HLöb" with "Hmodel Hslot HΦ").
+  Qed.
+  Lemma safe_dynarray_push_spec t vs v :
+    {{{
+      safe_dynarray_model t vs
+    }}}
+      safe_dynarray_push t v
+    {{{
+      RET #();
+      safe_dynarray_model t (vs ++ [v])
+    }}}.
+  Proof.
+    iIntros "%Φ Hmodel HΦ".
+    wp_rec. wp_alloc r as "Hr".
+    wp_smart_apply (safe_dynarray_try_push_spec with "[$Hmodel Hr]"); first iSmash. iIntros ([]); first iSmash. iIntros "(Hmodel & Hslot)".
+    wp_smart_apply (safe_dynarray_push_aux_spec with "[$Hmodel $Hslot]").
+    iSmash.
+  Qed.
+
+  Context τ `{!iType (iPropI Σ) τ}.
+
+  #[local] Definition slot_type :=
+    opt_type (reference_type τ).
+  Definition safe_dynarray_type t : iProp Σ :=
+    ∃ l,
+    ⌜t = #l⌝ ∗
+    inv nroot (
+      ∃ (sz : nat) cap data,
+      l.[size] ↦ #sz ∗
+      l.[data] ↦ data ∗ array_type slot_type cap data
+    ).
+  #[global] Instance safe_dynarray_type_itype :
+    iType _ safe_dynarray_type.
+  Proof.
+    split. apply _.
+  Qed.
+
+  Lemma safe_dynarray_create_type :
+    {{{ True }}}
+      safe_dynarray_create #()
+    {{{ t,
+      RET t;
+      safe_dynarray_type t
+    }}}.
+  Proof.
+    iIntros "%Φ _ HΦ".
+    wp_rec.
+    wp_apply (array_create_type slot_type with "[//]"). iIntros "%data Hdata_type".
+    iApply wp_fupd.
+    wp_apply (record2_make_spec with "[//]"). iIntros "%l (Hl & _)". iDestruct (record2_model_eq_1 with "Hl") as "(Hsz & Hdata)".
+    iSmash.
+  Qed.
+
+  Lemma safe_dynarray_make_type sz v :
+    {{{
+      int_type sz ∗
+      τ v
+    }}}
+      safe_dynarray_make sz v
+    {{{ t,
+      RET t;
+      safe_dynarray_type t
+    }}}.
+  Proof.
+    iIntros "%Φ ((%sz_ & ->) & #Hv) HΦ".
+    wp_rec.
+    wp_smart_apply assume_spec'. iIntros "%Hsz".
+    Z_to_nat sz_ as sz.
+    wp_smart_apply (array_init_type slot_type); first iSmash. iIntros "%data Hdata_type".
+    iApply wp_fupd.
+    wp_smart_apply (record2_make_spec with "[//]"). iIntros "%l (Hl & _)". iDestruct (record2_model_eq_1 with "Hl") as "(Hsz & Hdata)".
+    iSmash.
+  Qed.
+
+  Lemma safe_dynarray_size_type t :
+    {{{
+      safe_dynarray_type t
+    }}}
+      safe_dynarray_size t
+    {{{ (sz : nat),
+      RET #sz; True
+    }}}.
+  Proof.
+    iSmash.
+  Qed.
+
+  #[local] Lemma safe_dynarray_data_type t :
+    {{{
+      safe_dynarray_type t
+    }}}
+      safe_dynarray_data t
+    {{{ cap data,
+      RET data;
+      array_type slot_type cap data
+    }}}.
+  Proof.
+    iSmash.
+  Qed.
+
+  #[local] Lemma safe_dynarray_set_size_type t sz :
+    {{{
+      safe_dynarray_type t ∗
+      nat_type sz
+    }}}
+      safe_dynarray_set_size t sz
+    {{{
+      RET #(); True
+    }}}.
+  Proof.
+    iSmash.
+  Qed.
+
+  #[local] Lemma safe_dynarray_set_data_type t cap data :
+    {{{
+      safe_dynarray_type t ∗
+      array_type slot_type cap data
+    }}}
+      safe_dynarray_set_data t data
+    {{{
+      RET #(); True
+    }}}.
+  Proof.
+    iSmash.
+  Qed.
+
+  Lemma safe_dynarray_is_empty_type t :
+    {{{
+      safe_dynarray_type t
+    }}}
+      safe_dynarray_is_empty t
+    {{{ b,
+      RET #b; True
+    }}}.
+  Proof.
+    iSmash.
+  Qed.
+
+  Lemma safe_dynarray_get_type t (i : val) :
+    {{{
+      safe_dynarray_type t ∗
+      int_type i
+    }}}
+      safe_dynarray_get t i
+    {{{ v,
+      RET v;
+      τ v
+    }}}.
+  Proof.
+    iIntros "%Φ (#Htype & (%i_ & ->)) HΦ".
+    wp_rec.
+    wp_smart_apply (safe_dynarray_data_type with "Htype"). iIntros "%cap %data #Hdata_type".
+    wp_apply (array_get_type with "[$Hdata_type]"); first iSmash. iIntros "%v [-> | (%ref & -> & #Href)]".
+    - wp_smart_apply wp_diverge.
+    - wp_smart_apply (reference_get_type with "Href"). iSmash.
+  Qed.
+
+  Lemma safe_dynarray_set_type t (i : val) v :
+    {{{
+      safe_dynarray_type t ∗
+      int_type i ∗
+      τ v
+    }}}
+      safe_dynarray_set t i v
+    {{{
+      RET #(); True
+    }}}.
+  Proof.
+    iIntros "%Φ (#Htype & (%i_ & ->) & #Hv) HΦ".
+    wp_rec.
+    wp_smart_apply (safe_dynarray_data_type with "Htype"). iIntros "%cap %data #Hdata_type".
+    wp_apply (array_get_type with "[$Hdata_type]"); first iSmash. iIntros "%w [-> | (%ref & -> & #Href)]".
+    - wp_smart_apply wp_diverge.
+    - wp_smart_apply (reference_set_type with "[$Href $Hv]"). iSmash.
+  Qed.
+
+  Lemma safe_dynarray_reserve_type t n :
+    {{{
+      safe_dynarray_type t ∗
+      int_type n
+    }}}
+      safe_dynarray_reserve t n
+    {{{
+      RET #(); True
+    }}}.
+  Proof.
+    iIntros "%Φ (#Htype & (%n_ & ->)) HΦ".
+    wp_rec.
+    wp_smart_apply (safe_dynarray_data_type with "Htype"). iIntros "%cap %data #Hdata_type".
+    wp_smart_apply (array_size_type with "Hdata_type"). iIntros "_".
+    wp_pures.
+    case_bool_decide; wp_pures; first iSmash.
+    wp_apply assume_spec'. iIntros "%Hn".
+    wp_smart_apply (safe_dynarray_next_capacity_spec with "[//]"); first lia. iIntros "%n' %Hn'".
+    wp_apply maximum_spec.
+    wp_smart_apply (array_make_type slot_type); first iSmash. iIntros "%data' #Hdata_type'".
+    wp_smart_apply safe_dynarray_size_type; first iSmash+. iIntros "%sz _".
+    wp_smart_apply (array_blit_type slot_type); first iSmash. iIntros "_".
+    wp_smart_apply (safe_dynarray_set_data_type with "[$Htype $Hdata_type']"). iIntros "_".
+    iSmash.
+  Qed.
+  Lemma safe_dynarray_reserve_extra_type t n :
+    {{{
+      safe_dynarray_type t ∗
+      int_type n
+    }}}
+      safe_dynarray_reserve_extra t n
+    {{{
+      RET #(); True
+    }}}.
+  Proof.
+    iIntros "%Φ (#Htype & (%n_ & ->)) HΦ".
+    wp_rec. wp_pures.
+    case_bool_decide; wp_pures; last iSmash.
+    wp_apply (safe_dynarray_size_type with "Htype"). iIntros "%sz _".
+    wp_smart_apply (safe_dynarray_reserve_type with "[$Htype]"); first iSmash.
+    iSmash.
+  Qed.
+
+  #[local] Lemma safe_dynarray_try_push_type t slot :
+    {{{
+      safe_dynarray_type t ∗
+      slot_type slot
+    }}}
+      safe_dynarray_try_push t slot
+    {{{ b,
+      RET #b; True
+    }}}.
+  Proof.
+    iIntros "%Φ (#Htype & #Hslot) HΦ".
+    wp_rec.
+    wp_smart_apply (safe_dynarray_size_type with "Htype"). iIntros "%sz _".
+    wp_smart_apply (safe_dynarray_data_type with "Htype"). iIntros "%cap %data #Hdata_type".
+    wp_smart_apply (array_size_type with "Hdata_type"). iIntros "_".
+    wp_pures.
+    case_bool_decide; wp_pures; first iSmash.
+    wp_apply (array_unsafe_set_type with "[$Hdata_type $Hslot]"); first lia. iIntros "_".
+    wp_smart_apply (safe_dynarray_set_size_type with "[$Htype]"); first iSmash. iIntros "_".
+    iSmash.
+  Qed.
+  #[local] Lemma safe_dynarray_push_aux_type t slot :
+    {{{
+      safe_dynarray_type t ∗
+      slot_type slot
+    }}}
+      safe_dynarray_push_aux t slot
+    {{{
+      RET #(); True
+    }}}.
+  Proof.
+    iIntros "%Φ (#Htype & #Hslot) HΦ".
+    iLöb as "HLöb".
+    wp_rec.
+    wp_smart_apply (safe_dynarray_reserve_extra_type with "[$Htype]"); first iSmash. iIntros "_".
+    wp_smart_apply (safe_dynarray_try_push_type with "[$Htype $Hslot]"). iIntros ([]) "_"; first iSmash.
+    wp_smart_apply ("HLöb" with "HΦ").
+  Qed.
+  Lemma safe_dynarray_push_type t v :
+    {{{
+      safe_dynarray_type t ∗
+      τ v
+    }}}
+      safe_dynarray_push t v
+    {{{
+      RET #(); True
+    }}}.
+  Proof.
+    iIntros "%Φ (#Htype & #Hv) HΦ".
+    wp_rec. wp_alloc r as "Hr".
+    iAssert (|={⊤}=> slot_type (&&Some #r))%I with "[Hr]" as ">#Hslot"; first iSmash.
+    wp_smart_apply (safe_dynarray_try_push_type with "[$Htype $Hslot]"). iIntros ([]) "_"; first iSmash.
+    wp_smart_apply (safe_dynarray_push_aux_type with "[$Htype $Hslot]"). iIntros "_".
+    iSmash.
+  Qed.
+End heapGS.
+
+#[global] Opaque safe_dynarray_create.
+#[global] Opaque safe_dynarray_make.
+#[global] Opaque safe_dynarray_init.
+#[global] Opaque safe_dynarray_size.
+#[global] Opaque safe_dynarray_is_empty.
+#[global] Opaque safe_dynarray_get.
+#[global] Opaque safe_dynarray_set.
+#[global] Opaque safe_dynarray_reserve.
+#[global] Opaque safe_dynarray_reserve_extra.
+#[global] Opaque safe_dynarray_push.
+
+#[global] Opaque safe_dynarray_model.
+#[global] Opaque safe_dynarray_type.
